src/Eval.v
@@ -14,8 +14,6 @@ Generalizable All Variables.
 
 Import ListNotations.
 
-Section Eval.
-
 Reserved Notation " t '--->' t' " (at level 40).
 
 (************************************************************************
@@ -26,11 +24,11 @@ Inductive Step : ∀ {τ}, Exp [] τ → Exp [] τ → Prop :=
   | ST_Seq τ τ' (e1 : Exp [] τ') (e2 : Exp [] τ) :
     Seq e1 e2 ---> e2
 
-  | ST_ListElem τ (l : list (Exp [] τ)) l' pre post x x' :
-    l  = pre ++ x  :: post →
-    l' = pre ++ x' :: post →
+  | ST_ListElem τ (l1 l2 : list (Exp [] τ)) pre x x' post :
+    l1 = pre ++ x  :: post →
+    l2 = pre ++ x' :: post →
     x ---> x' →
-    List l ---> List l'
+    List l1 ---> List l2
 
   | ST_Let τ ty (x : Exp [] ty) (body : Exp [ty] τ) :
     Let x body ---> APP (LAM body) x
@@ -43,9 +41,10 @@ Inductive Step : ∀ {τ}, Exp [] τ → Exp [] τ → Prop :=
     e1 ---> e1' →
     APP e1 e2 ---> APP e1' e2
 
-  | ST_App dom cod (e1 : Exp [] (dom ⟶ cod)) (e2 : Exp [] dom) e2' :
+  | ST_App2 dom cod (v1 : Exp [] (dom ⟶ cod)) (e2 : Exp [] dom) e2' :
+    ValueP v1 →
     e2 ---> e2' →
-    APP e1 e2 ---> APP e1 e2'
+    APP v1 e2 ---> APP v1 e2'
 
   where " t '--->' t' " := (Step t t').
 
@@ -57,96 +56,223 @@ Proof.
   extensionality E;
   destruct E.
   - subst.
-    rewrite !map_app.
-    f_equal.
-    rewrite !map_cons.
-    f_equal.
-    now rewrite IHStep.
+    rewrite !map_app; f_equal.
+    rewrite !map_cons; f_equal.
+    now rewrite !IHStep.
   - now rewrite <- SemSubComm.
   - now rewrite IHStep.
   - now rewrite IHStep.
 Qed.
 
-Definition normal_form {X : Type}
-           (R : relation X) (t : X) : Prop :=
+Definition normal_form {X : Type} (R : relation X) (t : X) : Prop :=
   ¬ ∃ t', R t t'.
 
-Lemma app_cons A (y : A) (xs ys : list A) :
-  xs ++ y :: ys = (xs ++ [y]) ++ ys.
-Proof.
-  induction xs; simpl; auto.
-  now rewrite IHxs.
-Qed.
+Ltac reduce :=
+  repeat lazymatch goal with
+         | [ H : existT _ _ _ = existT _ _ _ |- _ ] =>
+             apply inj_pair2 in H; subst
+         | [ H : _ ∧ _ |- _ ] => destruct H
+         | [ H : _ * _ |- _ ] => destruct H
+         | [ H : ∃ _, _ |- _ ] => destruct H
+         end.
 
-Lemma value_is_nf {τ} (v : Exp [] τ) :
+Ltac inv H := inversion H; subst; clear H; reduce.
+
+Theorem value_is_nf {τ} (v : Exp [] τ) :
   ValueP v → normal_form Step v.
 Proof.
   intros.
-  induction H; intro.
-  - destruct H.
-    now inversion H.
-  - destruct H0.
-    generalize dependent x.
-    induction H; intros.
-    + inversion H0.
-      apply inj_pair2 in H1, H2; subst.
-      apply app_eq_nil in H1.
-      destruct H1.
+  unfold normal_form.
+  dependent induction v using Exp_rect';
+  inv H; intro; reduce.
+  - now inversion H.
+  - induction l; simpl in *.
+    + inv H.
+      destruct pre; simpl in *;
       now inversion H1.
-    + inversion H1.
-      apply inj_pair2 in H3, H4; subst.
-      destruct pre.
-      * simpl in *.
-        inversion H3; subst.
-        admit.
+    + reduce.
+      inv H2.
+      intuition.
+      inv H.
+      destruct pre; simpl in *.
+      * inv H2.
+        now eapply n; eauto.
       * admit.
-  - destruct H.
-    now inversion H.
-Abort.
-
-Theorem strong_progress {τ} (e : Exp [] τ) :
-  ValueP e ∨ ∃ e', e ---> e'.
-Proof.
-  dependent elimination e.
-  - now left; constructor.
-  - right.
-    eexists e0.
-    now constructor.
-  - induction l0; simpl.
-    + now left; constructor.
-    + destruct IHl0.
-      * destruct (classic (ValueP a)).
-        ** left.
-           constructor.
-           *** constructor; auto.
-               inversion H; subst.
-               apply inj_pair2 in H2.
-               now subst.
-        ** right.
-           admit.
-      * destruct H.
-        inversion H; subst.
-        apply inj_pair2 in H1; subst.
-        apply inj_pair2 in H2; subst.
-        right.
-        exists (List (a :: pre ++ x' :: post)).
-        rewrite !app_comm_cons.
-        now eapply ST_ListElem; eauto.
-Abort.
+  - now inversion H.
+Admitted.
 
 Definition deterministic {X : Type} (R : relation X) :=
   ∀ x y1 y2 : X, R x y1 → R x y2 → y1 = y2.
 
 Theorem step_deterministic τ :
   deterministic (@Step τ).
-Abort.
+Proof.
+  repeat intro.
+  induction H.
+  - now inv H0.
+  - subst.
+    inv H0.
+    admit.
+  - now inv H0.
+  - inv H0; auto.
+    + now inversion H3.
+    + apply value_is_nf in H.
+      destruct H.
+      now exists e2'.
+  - inv H0.
+    + now inversion H.
+    + f_equal.
+      now apply IHStep.
+    + apply value_is_nf in H4.
+      destruct H4.
+      now exists e1'.
+  - inv H0.
+    + apply value_is_nf in H4.
+      destruct H4.
+      now exists e2'.
+    + apply value_is_nf in H.
+      destruct H.
+      now exists e1'.
+    + f_equal.
+      now apply IHStep.
+Admitted.
 
-Lemma nf_is_value τ (v : Exp [] τ) :
+Theorem strong_progress {τ} (e : Exp [] τ) :
+  ValueP e ∨ ∃ e', e ---> e'.
+Proof.
+  dependent induction e using Exp_rect'.
+  - now left; constructor.
+  - right.
+    eexists e2.
+    now constructor.
+  - induction l; simpl in *.
+    + left.
+      now constructor.
+    + destruct X.
+      destruct (o _ eq_refl JMeq_refl).
+      * intuition.
+        ** left.
+           constructor.
+           inv H1.
+           now constructor.
+        ** right.
+           destruct H1.
+           inv H0.
+           exists (List (a :: pre ++ x' :: post)).
+           now apply ST_ListElem
+             with (pre:=a :: pre) (post:=post) (x:=x0) (x':=x'); auto.
+      * right.
+        destruct H.
+        exists (List (x :: l)).
+        now apply ST_ListElem
+          with (pre:=[]) (post:=l) (x:=a) (x':=x); auto.
+  - right.
+    exists (APP (LAM e2) e1).
+    now constructor.
+  - now inversion v.
+  - left.
+    now constructor.
+  - right.
+    destruct (IHe1 _ eq_refl JMeq_refl); clear IHe1.
+    + destruct (IHe2 _ eq_refl JMeq_refl); clear IHe2.
+      * dependent elimination e1; inv H.
+        exists (STmExp {| e2 |} e4).
+        now constructor.
+      * dependent elimination e1; inv H.
+        exists (APP (LAM e4) x).
+        constructor; auto.
+        now constructor.
+    + reduce.
+      destruct (IHe2 _ eq_refl JMeq_refl); clear IHe2.
+      * exists (APP x e2).
+        now constructor.
+      * reduce.
+        exists (APP x e2).
+        now constructor.
+Qed.
+
+Corollary nf_is_value τ (v : Exp [] τ) :
   normal_form Step v → ValueP v.
-Abort.
+Proof.
+  intros.
+  destruct (strong_progress v); auto.
+  exfalso.
+  now apply H.
+Qed.
 
 Corollary nf_same_as_value τ (v : Exp [] τ) :
   normal_form Step v ↔ ValueP v.
-Abort.
+Proof.
+  split.
+  - now apply nf_is_value.
+  - now apply value_is_nf.
+Qed.
 
-End Eval.
+Inductive multi {X : Type} (R : relation X) : relation X :=
+  | multi_refl : ∀ (x : X), multi R x x
+  | multi_step : ∀ (x y z : X),
+      R x y →
+      multi R y z →
+      multi R x z.
+
+Notation " t '--->*' t' " := (multi Step t t') (at level 40).
+
+Theorem multi_R : ∀ (X : Type) (R : relation X) (x y : X),
+  R x y → (multi R) x y.
+Proof.
+  intros.
+  eapply multi_step; eauto.
+  now constructor.
+Qed.
+
+Theorem multi_trans : ∀ (X : Type) (R : relation X) (x y z : X),
+  multi R x y →
+  multi R y z →
+  multi R x z.
+Proof.
+  intros.
+  induction H; auto.
+  now eapply multi_step; eauto.
+Qed.
+
+Definition halts {τ} (e : Exp [] τ) : Prop :=
+  ∃ e', e --->* e' ∧ ValueP e'.
+
+Lemma value_halts {τ} (v : Exp [] τ) : ValueP v → halts v.
+Proof.
+  intros.
+  unfold halts.
+  now dependent induction H; eexists; split; constructor.
+Qed.
+
+Lemma step_preserves_halting {τ} (e e' : Exp [] τ) :
+  (e ---> e') → (halts e ↔ halts e').
+Proof.
+  intros.
+  unfold halts.
+  split.
+  - intros [e'' [H1 H2]].
+    destruct H1.
+    + apply value_is_nf in H2.
+      destruct H2.
+      now exists e'.
+    + rewrite (step_deterministic _ _ _ _ H H0).
+      now exists z.
+  - intros [e'0 [H1 H2]].
+    exists e'0.
+    split; auto.
+    now eapply multi_step; eauto.
+Qed.
+
+Definition normal_form_of {τ} (e e' : Exp [] τ) :=
+  (e --->* e' ∧ normal_form Step e').
+
+Theorem normal_forms_unique τ :
+  deterministic (normal_form_of (τ:=τ)).
+Proof.
+  unfold normal_form_of, normal_form.
+  repeat intro.
+Admitted.
+
+Definition normalizing {X : Type} (R : relation X) :=
+  ∀ t, ∃ t', (multi R) t t' ∧ normal_form R t'.
